Typed stack machine with proofs completed

CpdtLean/StackMachine.lean
@@ -11,6 +11,7 @@ inductive Instr : Type where
 
 abbrev Prog := List Instr
 abbrev Stack := List Nat
+
 end Types
 
 open Types
@@ -53,8 +54,7 @@ def compile (e : Exp) : Prog :=
   | Exp.const n => (Instr.iConst n)::[]
   | Exp.binop b e1 e2 => compile e2 ++ compile e1 ++ (Instr.iBinop b ::[])
 
--- Don't know why I added this proof but a good exercise
-theorem nonEmptyProgramIfCompiled (e: Exp) : List.length (compile e) >= 1 :=  by
+@[simp] theorem nonEmptyProgramIfCompiled (e: Exp) : List.length (compile e) >= 1 :=  by
   induction e with
   | const a =>
     unfold compile
@@ -102,10 +102,173 @@ theorem compile_correct' : ∀ e p s, progDenote (compile e ++ p) s = progDenote
             }
 
 
-theorem compile_correct : ∀ (e: Exp) , progDenote (compile e) [] = Option.some ((expDenote e) :: []) := by {
+theorem compile_correct : ∀ (e: Exp) ,
+progDenote (compile e) [] = Option.some ((expDenote e) :: []) := by {
   intro e
   rw [←List.append_nil (compile e)]
   rw [compile_correct']
   unfold progDenote
   rfl
 }
+
+
+namespace Types
+
+-- nat or a bool is a type
+inductive Typ where
+  | nat
+  | bool
+
+-- types of binary operations, parameterized over the Typ
+inductive TBinop: Typ -> Typ -> Typ -> Type where
+  | tplus : TBinop .nat .nat .nat
+  | ttimes : TBinop .nat .nat .nat
+  | teq: forall t, TBinop t t .bool -- eq defined to be over any type
+  | tlt : TBinop .nat .nat .bool
+
+-- type of an expression
+inductive TExp: Typ -> Type where
+  | tnconst : Nat -> TExp .nat
+  | tbconst : Bool -> TExp .bool
+  | tbinop : forall t1 t2 t, TBinop t1 t2 t -> TExp t1 -> TExp t2 -> TExp t
+
+-- type stack, just a stack maintaining the current type at the top?
+abbrev TStack := List Typ
+
+-- type of an instruction, parameterized over the old type stack and new type stack (TInstr: old_type_stack -> new_type_stack)
+inductive TInstr : TStack -> TStack -> Type where
+  | ti_nconst : forall s, Nat -> TInstr s (.nat::s)
+  | ti_bconst : forall s, Bool -> TInstr s (.bool::s)
+  | ti_binop : forall arg1 arg2 res s, TBinop arg1 arg2 res -> TInstr (arg1::arg2::s) (res::s)
+
+-- type of a program, parameterized over the previous type stack and new type stack
+inductive TProg : TStack -> TStack -> Type where
+  -- program is unchanged
+  | tnil : forall s, TProg s s
+  -- takes an instruction(s1 -> s2), program(s2 -> s3), which results in a
+  -- program (s1 -> s3). During interpretation, we process the instruction first
+  -- and the rest of the program.
+  | tcons : forall s1 s2 s3, TInstr s1 s2 -> TProg s2 s3 -> TProg s1 s3
+
+end Types
+
+-- convert our Typ to a Lean Type
+def typeDenote (t: Typ) :=
+    match t with
+    | .nat => Nat
+    | .bool => Bool
+
+
+-- convert a TBinop to a Lean binary function
+def tbinopDenote { arg1 arg2 res :Typ}
+    (b: TBinop arg1 arg2 res) : typeDenote arg1 -> typeDenote arg2 -> typeDenote res :=
+  match b with
+  | .tplus => Nat.add
+  | .ttimes => Nat.mul
+  -- Cannot find a better way to do this,
+  -- possibly refactor this
+  | .tlt => (fun ( x y:Nat ) =>
+        match ( Ord.compare x y ) with
+        | .lt => true
+        | _ => false
+      )
+  | .teq .nat => fun ( x y:Nat ) =>
+        match ( Ord.compare x y ) with
+        | .eq => true
+        | _ => false
+  | .teq .bool => fun ( x y:Bool) =>
+
+        match ( Ord.compare x y ) with
+        | .eq => true
+        | _ => false
+
+-- interpret a TExp
+def texpDenote {t: Typ} (e: TExp t) : typeDenote t :=
+  match e with
+  | .tnconst n => n
+  | .tbconst b => b
+  | .tbinop _ _ _ b e1 e2 => (tbinopDenote b) (@texpDenote _ e1) (@texpDenote _ e2)
+
+
+
+#check texpDenote
+#eval texpDenote (.tnconst 20)
+#eval texpDenote (.tbinop _ _ _ .tlt (.tnconst 10) (.tnconst 20) )
+#eval texpDenote (.tbinop _ _ _ (.teq .nat) (.tnconst 20) (.tnconst 20) )
+#eval texpDenote (.tbinop _ _ _ (.teq .nat) (.tnconst 21) (.tnconst 20) )
+
+
+-- TStack(type stack) to Lean Types
+def vstack (ts: TStack) : Type :=
+    match ts with
+    | List.nil => Unit
+    | t::ts => typeDenote t × vstack ts
+
+-- Interpret a TInstr. Takes in a TInstr, the value stack(based on type stack)
+-- and reads a new value stack
+def tinstrDenote { ts ts': TStack } (i: TInstr ts ts') : vstack ts -> vstack ts' :=
+    match i with
+    | TInstr.ti_nconst _ n => fun s => (n,s)
+    | TInstr.ti_bconst _ b => fun s => (b,s)
+    | TInstr.ti_binop _ _ _  _ binop => fun s =>
+      let (arg1, (arg2, rest)) := s
+      ((tbinopDenote binop arg1 arg2), rest)
+
+
+-- Interpret a TProg. Takes in a TProg and then value stack and returns a new value stack
+def tprogDenote {ts ts': TStack} (p: TProg ts ts') : vstack ts -> vstack ts' :=
+    match p with
+    -- Do nothing
+    | TProg.tnil _ => fun s => s
+    -- Interpret instr and then rest of the program
+    | TProg.tcons _ _ _ instr prog' => fun s => tprogDenote prog' (tinstrDenote instr s)
+
+
+def tconcat { ts ts' ts'': TStack } (p: TProg ts ts') : TProg ts' ts'' -> TProg ts ts'' :=
+    match p with
+    -- Do nothing
+    | TProg.tnil _ => fun p => p
+    -- drains the instructions of p and then adds instructions of p'
+    | TProg.tcons _ _ _ instr rest => fun p' => TProg.tcons _ _ _ instr (tconcat rest p')
+
+def tcompile { t: Typ } (e: TExp t) (ts: TStack) : TProg ts (t::ts) :=
+    match e with
+    | TExp.tbconst b => TProg.tcons _ _ _ (TInstr.ti_bconst _ b) ( .tnil _)
+    | TExp.tnconst n => TProg.tcons _ _ _ (TInstr.ti_nconst _ n) (.tnil _)
+    | TExp.tbinop _ _ _ op arg1 arg2 =>
+    -- needs to be compiled in a way so that we have arg2, arg1 in stack and
+    -- then apply the binary operation, hence this way ([arg2][arg1][<op>])
+      tconcat (tcompile arg2 _)
+              (tconcat (tcompile arg1 _)
+                       (.tcons _ _ _ (.ti_binop _ _ _ _ op) (.tnil _)))
+
+#eval tprogDenote (tcompile (.tnconst 42) .nil) Unit.unit
+
+theorem tprogDenote_over_tconcat :
+          forall ts ts' ts'' ( p1: TProg ts ts' ) ( p2: TProg ts' ts'' ) (vs: vstack ts),
+          tprogDenote (tconcat p1 p2) vs = tprogDenote p2 (tprogDenote p1 vs) := by
+    intro ts ts' ts'' p1
+    induction p1 with
+    | tnil => intro p2 vs; rfl
+    | tcons _ _ _ instr prog IH =>
+      intro p2 vs; unfold tconcat;
+      conv => lhs;unfold tprogDenote; rw [IH]
+      conv => rhs; arg 2; unfold tprogDenote;
+      done
+
+theorem tcompile_correct : forall t (e: TExp t) ts (s: vstack ts),
+      tprogDenote (tcompile e ts) s  = (texpDenote e, s) := by
+    intros t e ts s
+    induction e generalizing ts s with
+    | tnconst => unfold tcompile texpDenote; rfl
+    | tbconst => unfold tcompile texpDenote; rfl
+    | tbinop _ _ _ op e1 e2 IHe1 IHe2 =>
+      unfold tcompile; unfold texpDenote;
+      rw [tprogDenote_over_tconcat ]
+
+      rw [tprogDenote_over_tconcat ]
+      conv => lhs; unfold tprogDenote;  simp; rw [IHe2, IHe1]
+      unfold tprogDenote
+      conv => rhs;
+      rfl
+      done
